---
title: "General Equation of a Straight Line"
author: emanetat
description: 
date: 2023-07-24T16:06:50+08:00
draft: false
weight: 
hidemeta: false

cover:
    image: "<image path/url>" # image path/url
    alt: "<alt text>" # alt text
    caption: "<text>" # display caption under cover
    relative: false # when using page bundles set this to true
    hidden: true # only hide on current single page

categories: []
tags: [math, test]

comments: false
---
$$ (x - x_1)/(x_2 - x_1) = (y - y_1)/(y_2-y_1) $$

$$ (y_2 - y_1)x - (x_2 - x_1)y - x_1 \ast x_2 + y_1 \ast x_2 = 0 $$

coefficient will be:

- $ a = y_2 - y_1 $
- $ b = -(x_2 - x_1) = x_1 - x_2 $
- $ c = y1 \ast x2 - x1 \ast y2 $
